Define the memory machine

Basic.v
@@ -3,12 +3,57 @@ Require Import PArith.
 Require Import FMapPositive.
 Require Import MSetPositive.
 
+Set Implicit Arguments.
+
+Module PositiveFun.
+  Section PositiveFun.
+    Variable (V:Type).
+
+    Structure t := mk {
+      map: PositiveMap.t V;
+      default: V;
+    }.
+
+    Definition empty (v:V) := mk (PositiveMap.empty _) v.
+
+    Definition find (p:positive) (f:t): V :=
+      match PositiveMap.find p f.(map) with
+      | Some v => v
+      | None => f.(default)
+      end.
+
+    Definition add (p:positive) (v:V) (f:t): t :=
+      mk
+        (PositiveMap.add p v f.(map))
+        f.(default).
+
+    Lemma empty_spec p v:
+      find p (empty v) = v.
+    Proof.
+      unfold find, empty. simpl.
+      rewrite PositiveMap.gempty. auto.
+    Qed.
+
+    Lemma add_spec p' p v f:
+      find p' (add p v f) =
+      if Pos.eq_dec p' p
+      then v
+      else find p' f.
+    Proof.
+      unfold find, add. simpl.
+      rewrite PositiveMapAdditionalFacts.gsspec.
+      destruct (PositiveMap.E.eq_dec p' p), (Pos.eq_dec p' p); congruence.
+    Qed.
+  End PositiveFun.
+End PositiveFun.
+
 Module Ident.
   Definition t := Pos.t.
   Definition eq_dec := Pos.eq_dec.
 
   Module Map := PositiveMap.
   Module Set_ := PositiveSet.
+  Module Fun := PositiveFun.
 
   Parameter of_string: String.string -> t.
   Hypothesis of_string_inject:
