Memory.v
@@ -1,0 +1,137 @@
+Require Import Equalities.
+Require Import MSetWeakList.
+Require Import PeanoNat.
+
+Require Import Basic.
+Require Import Event.
+Require Import Program.
+
+Set Implicit Arguments.
+
+Module LocalClock.
+  Definition t := Loc.Fun.t nat.
+
+  Definition empty := Loc.Fun.empty 0.
+
+  Definition le (lhs rhs:t): Prop :=
+    forall loc, Loc.Fun.find loc lhs <= Loc.Fun.find loc rhs.
+End LocalClock.
+
+Module Clock.
+  Definition t := Ident.Fun.t LocalClock.t.
+
+  Definition empty := Ident.Fun.empty LocalClock.empty.
+
+  Definition le (lhs rhs:t): Prop :=
+    forall i, LocalClock.le (Ident.Fun.find i lhs) (Ident.Fun.find i rhs).
+End Clock.
+
+Module Message <: DecidableType.
+  Structure t_ := mk {
+    event: Event.t;
+    timestamp: nat;
+  }.
+  Definition t := t_.
+
+  Definition eq := @eq t.
+  Program Instance eq_equiv: Equivalence eq.
+  Definition eq_dec (x y:t): {eq x y} + {~ eq x y}.
+  Proof.
+    unfold eq.
+    decide equality;
+      (try apply Event.eq_dec);
+      (try apply Nat.eq_dec).
+  Qed.
+End Message.
+
+Module MessageSet := MSetWeakList.Make (Message).
+
+Module Buffer.
+  Structure t := mk {
+    history: list Message.t;
+    inception: MessageSet.t;
+  }.
+
+  Definition empty := mk nil MessageSet.empty.
+
+  Inductive position :=
+  | h (n:nat)
+  | i
+  .
+
+  Inductive In (msg:Message.t) (b:t): forall (p:position), Prop :=
+  | In_history
+      n
+      (HISTORY: List.nth_error b.(history) n = Some msg):
+      In msg b (h n)
+  | In_inception
+      (INCEPTION: MessageSet.In msg b.(inception)):
+      In msg b i
+  .
+
+  Definition add_inception (msg:Message.t) (b:t): t :=
+    mk b.(history) (MessageSet.add msg b.(inception)).
+End Buffer.
+
+Module Memory.
+  Definition t := Ident.Fun.t Buffer.t.
+
+  Definition empty := Ident.Fun.empty Buffer.empty.
+
+  Definition position := (Ident.t * Buffer.position)%type.
+
+  Inductive In (msg:Message.t) (m:t): forall (p:position), Prop :=
+  | In_intro
+      i p
+      (IN: Buffer.In msg (Ident.Fun.find i m) p):
+      In msg m (i, p)
+  .
+
+  (* TODO *)
+  Inductive step (c:Clock.t): forall (s1:t) (i:Ident.t) (e:option Event.t) (s2:t), Prop :=
+  .
+End Memory.
+
+Module State.
+  Structure t := mk {
+    clock: Clock.t;
+    program: Program.t;
+    memory: Memory.t;
+    stack: list (Program.t * Memory.t);
+  }.
+
+  Inductive step: forall (s1 s2:t), Prop :=
+  | step_event
+      i e
+      c p1 p2 m1 m2 stack
+      (PROGRAM: Program.step p1 i e p2)
+      (MEMORY: Memory.step c m1 i e m2):
+      step (mk c p1 m1 stack) (mk c p2 m2 stack)
+  | step_dream
+      c p m stack:
+      step (mk c p m stack) (mk c p m ((p, m)::stack))
+  | step_inception
+      c p m p' m' stack
+      event ts ts' position i
+      (MESSAGE: Memory.In (Message.mk event ts) m position)
+      (POSITION: position.(snd) <> Buffer.i)
+      (INCEPTION:
+         forall i,
+           MessageSet.Subset
+             (Ident.Fun.find i m).(Buffer.inception)
+             (Ident.Fun.find i m').(Buffer.inception)):
+      step
+        (mk c p m ((p', m')::stack))
+        (mk c
+            p'
+            (Ident.Fun.add i (Buffer.add_inception (Message.mk event ts') (Ident.Fun.find i m')) m')
+            stack)
+  | step_commit
+      c p m c'
+      (MEMORY: forall i, MessageSet.Empty (Ident.Fun.find i m).(Buffer.inception))
+      (CLOCK: Clock.le c c'):
+      step
+        (mk c p m nil)
+        (mk c' p m nil)
+  .
+End State.
