Program.v
@@ -1,0 +1,48 @@
+Require Import Basic.
+Require Import Event.
+
+Set Implicit Arguments.
+
+Module Language.
+  Structure t := mk {
+    state: Type;
+    is_terminal: state -> Prop;
+    step: forall (s1:state) (e:option Event.t) (s2:state), Prop;
+  }.
+End Language.
+
+Module Thread.
+  Structure t := mk {
+    lang: Language.t;
+    state: lang.(Language.state)
+  }.
+
+  Definition is_terminal (th:t): Prop :=
+    th.(lang).(Language.is_terminal) th.(state).
+
+  Inductive step: forall (t1:t) (e:option Event.t) (t2:t), Prop :=
+  | step_intro
+      lang s1 e s2
+      (STEP: lang.(Language.step) s1 e s2):
+      step (mk lang s1) e (mk lang s2).
+End Thread.
+
+Module Program.
+  Definition t := Ident.Map.t Thread.t.
+
+  Inductive is_terminal (p:t): Prop :=
+  | is_terminal_intro
+      (TERMINAL:
+         forall i th
+           (S: Ident.Map.find i p = Some th),
+           Thread.is_terminal th)
+  .
+
+  Inductive step: forall (p1:t) (i:Ident.t) (e:option Event.t) (p1:t), Prop :=
+  | step_intro
+      p1 i th1 e th2
+      (TH1: Ident.Map.find i p1 = Some th1)
+      (STEP: Thread.step th1 e th2):
+      step p1 i e (Ident.Map.add i th2 p1)
+  .
+End Program.
