Semantics.v
@@ -1,0 +1,94 @@
+Require Import Event.
+Require Import Syntax.
+Require Import Thread.
+
+Set Implicit Arguments.
+
+Module RegSet.
+  Definition t := Reg.Fun.t Const.t.
+
+  Definition empty := Reg.Fun.empty Const.zero.
+
+  Definition eval_value (rs:t) (val:Value.t): Const.t :=
+    match val with
+    | Value.reg r => Reg.Fun.find r rs
+    | Value.const c => c
+    end.
+
+  Definition eval_rhs (rs:t) (rhs:Instr.rhs): Const.t :=
+    match rhs with
+    | Instr.rhs_val val => eval_value rs val
+    | Instr.rhs_op1 op op1 => Op1.eval op (eval_value rs op1)
+    | Instr.rhs_op2 op op1 op2 => Op2.eval op (eval_value rs op1) (eval_value rs op2)
+    end.
+End RegSet.
+
+Module Semantics.
+  Structure state: Type := mk {
+    regs: RegSet.t;
+    stmts: list Stmt.t;
+  }.
+
+  Definition is_terminal (s:state): Prop :=
+    stmts s = nil.
+
+  Inductive eval_instr: forall (rs1:RegSet.t) (i:Instr.t) (e:option Event.t) (rs2:RegSet.t), Prop :=
+  | eval_load
+      rs lhs rhs ord val:
+      eval_instr
+        rs
+        (Instr.load lhs rhs ord)
+        (Some (Event.read rhs val ord))
+        (Reg.Fun.add lhs val rs)
+  | eval_store
+      rs lhs rhs ord:
+      eval_instr
+        rs
+        (Instr.store lhs rhs ord)
+        (Some (Event.write lhs (RegSet.eval_value rs rhs) ord))
+        rs
+  | eval_fetch_add
+      rs lhs loc addendum ord val:
+      eval_instr
+        rs
+        (Instr.fetch_add lhs loc addendum ord)
+        (Some (Event.update loc val (Const.add val (RegSet.eval_value rs addendum)) ord))
+        (Reg.Fun.add lhs val rs)
+  | eval_assign
+      rs lhs rhs:
+      eval_instr
+        rs
+        (Instr.assign lhs rhs)
+        None
+        (Reg.Fun.add lhs (RegSet.eval_rhs rs rhs) rs)
+  .
+
+  Inductive step: forall (s1:state) (e:option Event.t) (s1:state), Prop :=
+  | step_instr
+      rs1 i e rs2 stmts
+      (INSTR: eval_instr rs1 i e rs2):
+      step
+        (mk rs1 ((Stmt.instr i)::stmts))
+        e
+        (mk rs2 stmts)
+  | step_ite
+      rs cond s1 s2 stmts:
+      step
+        (mk rs ((Stmt.ite cond s1 s2)::stmts))
+        None
+        (mk rs ((if RegSet.eval_value rs cond
+                 then s1
+                 else s2) ++ stmts))
+  | step_dowhile
+      rs s cond stmts:
+      step
+        (mk rs ((Stmt.dowhile s cond)::stmts))
+        None
+        (mk rs (s ++ (Stmt.ite cond (cons (Stmt.dowhile s cond) nil) nil) :: stmts))
+  .
+
+  Definition lang :=
+    Language.mk
+      is_terminal
+      step.
+End Semantics.
